theories/eris/total_primitive_laws.v
@@ -138,14 +138,11 @@ Proof.
   iIntros (σ1) "(Hh & Ht) !# /=".
   solve_red.
   iIntros (e2 σ2 Hs); inv_head_step.
-(*
-  iMod (ghost_map_insert (fresh_loc σ1.(tapes)) with "Ht") as "[$ Hl]".
+  iMod (primitive_laws.tapes_insert (fresh_loc σ1.(tapes)) with "Ht") as "[$ Hl]".
   { apply not_elem_of_dom, fresh_loc_is_fresh. }
   iFrame. iModIntro.
   by iApply "HΦ".
 Qed.
-*)
-  Admitted.
 
 Lemma twp_rand_tape N α n ns z E s :
   TCEq N (Z.to_nat z) →
@@ -154,17 +151,14 @@ Proof.
   iIntros (-> Φ) "Hl HΦ".
   iApply twp_lift_atomic_head_step; [done|].
   iIntros (σ1) "(Hh & Ht) !#".
-Admitted.
-(*
-  iDestruct (ghost_map_lookup with "Ht Hl") as %?.
+  iDestruct (tapes_lookup with "Ht Hl") as %?.
   solve_red.
   iIntros (e2 σ2 Hs).
   inv_head_step.
-  iMod (ghost_map_update with "Ht Hl") as "[$ Hl]".
+  iMod (tapes_update with "Ht Hl") as "[$ Hl]".
   iFrame. iModIntro.
   by iApply "HΦ".
 Qed.
-*)
 
 Lemma twp_rand_tape_empty N z α E s :
   TCEq N (Z.to_nat z) →
@@ -173,16 +167,13 @@ Proof.
   iIntros (-> Φ) "Hl HΦ".
   iApply twp_lift_atomic_head_step; [done|].
   iIntros (σ1) "(Hh & Ht) !#".
-Admitted.
-(*
-  iDestruct (ghost_map_lookup with "Ht Hl") as %?.
+  iDestruct (tapes_lookup with "Ht Hl") as %?.
   solve_red.
   iIntros (e2 σ2 Hs).
   inv_head_step.
   iFrame.
   iModIntro. iApply ("HΦ" with "[$Hl //]").
 Qed.
-*)
 
 Lemma twp_rand_tape_wrong_bound N M z α E ns s :
   TCEq N (Z.to_nat z) →
@@ -192,9 +183,7 @@ Proof.
   iIntros (-> ? Φ) "Hl HΦ".
   iApply twp_lift_atomic_head_step; [done|].
   iIntros (σ1) "(Hh & Ht) !#".
-Admitted.
-(*
-  iDestruct (ghost_map_lookup with "Ht Hl") as %?.
+  iDestruct (tapes_lookup with "Ht Hl") as %?.
   solve_red.
   iIntros (e2 σ2 Hs).
   inv_head_step.
@@ -202,7 +191,6 @@ Admitted.
   iModIntro.
   iApply ("HΦ" with "[$Hl //]").
 Qed.
-*)
 
 
 (** A rule for error amplification for recursive functions *)
